@prefix : <http://www.semanticweb.org/exam-example#> .
@prefix owl: <http://www.w3.org/2002/07/owl#> .
@prefix rdf: <http://www.w3.org/1999/02/22-rdf-syntax-ns#> .
@prefix xml: <http://www.w3.org/XML/1998/namespace> .
@prefix xsd: <http://www.w3.org/2001/XMLSchema#> .
@prefix rdfs: <http://www.w3.org/2000/01/rdf-schema#> .
@base <http://www.semanticweb.org/exam-example> .

<http://www.semanticweb.org/exam-example> rdf:type owl:Ontology .

#################################################################
#    Object Properties
#################################################################

###  http://www.semanticweb.org/exam-example#containsArticle
:containsArticle rdf:type owl:ObjectProperty ;
                 owl:inverseOf :isCollectedIn ;
                 rdfs:domain :OpenAccessRepository ;
                 rdfs:range :Article ;
                 rdfs:comment "containsArticle relates a repository to an article contained in it." .


###  http://www.semanticweb.org/exam-example#hasAbstract
:hasAbstract rdf:type owl:ObjectProperty ;
             rdfs:subPropertyOf :hasPart ;
             owl:inverseOf :isAbstractOf ;
             rdf:type owl:FunctionalProperty ;
             rdfs:domain :Article ;
             rdfs:range :Abstract ;
             rdfs:comment "hasAbstract is a subproperty of hasPart and relates an article to its abstract." .


###  http://www.semanticweb.org/exam-example#hasArticle
:hasArticle rdf:type owl:ObjectProperty ;
            rdfs:subPropertyOf :hasPart ;
            owl:inverseOf :isArticleOf ;
            rdfs:domain :JournalVolume ;
            rdfs:range :JournalArticle ;
            rdfs:comment "hasArticle is a subproperty of hasPart and relates a journal volume to its journal articles." .


###  http://www.semanticweb.org/exam-example#hasExtendedVersion
:hasExtendedVersion rdf:type owl:ObjectProperty ;
                    owl:inverseOf :isExtendedVersionOf ;
                    rdf:type owl:FunctionalProperty ,
                             owl:InverseFunctionalProperty ;
                    rdfs:domain :ConferenceArticle ;
                    rdfs:range :JournalArticle ;
                    rdfs:comment "hasExtendedVersion relates a conference article to the journal article extended by it." .


###  http://www.semanticweb.org/exam-example#hasIssue
:hasIssue rdf:type owl:ObjectProperty ;
          owl:inverseOf :isIssueOf ;
          rdf:type owl:InverseFunctionalProperty ;
          rdfs:domain :Journal ;
          rdfs:range :JournalVolume ;
          rdfs:comment "hasIssue relates a journal to the journal volumes that are its issues." .


###  http://www.semanticweb.org/exam-example#hasPart
:hasPart rdf:type owl:ObjectProperty ,
                  owl:TransitiveProperty ,
                  owl:ReflexiveProperty ;
         rdfs:comment "hasPart is a superproperty of: hasSection, hasArticle, hasAbstract." .


###  http://www.semanticweb.org/exam-example#hasReferences
:hasReferences rdf:type owl:ObjectProperty ;
               owl:inverseOf :refersTo ;
               rdfs:domain :Article ;
               rdfs:range :References .


###  http://www.semanticweb.org/exam-example#hasSection
:hasSection rdf:type owl:ObjectProperty ;
            rdfs:subPropertyOf :hasPart ;
            owl:inverseOf :isSectionOf ;
            rdfs:domain :Article ;
            rdfs:range :Section ;
            rdfs:comment "hasSection is a subproperty of hasPart and relates an article to its sections." .


###  http://www.semanticweb.org/exam-example#isAbstractOf
:isAbstractOf rdf:type owl:ObjectProperty ;
              rdfs:subPropertyOf :isPartOf ;
              rdf:type owl:InverseFunctionalProperty ;
              rdfs:domain :Abstract ;
              rdfs:range :Article ;
              rdfs:comment "isAbstractOf is a subproperty of isPartOf and relates an abstract to its article." .


###  http://www.semanticweb.org/exam-example#isArticleOf
:isArticleOf rdf:type owl:ObjectProperty ;
             rdfs:subPropertyOf :isPartOf ;
             rdfs:domain :JournalArticle ;
             rdfs:range :JournalVolume ;
             rdfs:comment "isArticleOf is a subproperty of isPartOf and relates an article to its journal volume." .


###  http://www.semanticweb.org/exam-example#isCollectedIn
:isCollectedIn rdf:type owl:ObjectProperty ;
               rdfs:domain :Article ;
               rdfs:range :OpenAccessRepository ;
               owl:propertyChainAxiom ( :isArticleOf
                                        :isIssueOf
                                        :isPublishedBy
                                        :usesRepository
                                      ) ;
               rdfs:comment "isCollectedIn relates an article to the open access repository in which it is collected." .


###  http://www.semanticweb.org/exam-example#isExtendedVersionOf
:isExtendedVersionOf rdf:type owl:ObjectProperty ,
                              owl:FunctionalProperty ,
                              owl:InverseFunctionalProperty ;
                     rdfs:domain :JournalArticle ;
                     rdfs:range :ConferenceArticle ;
                     rdfs:comment "isExtendedVersionOf relates a journal article to the conference article it extends." .


###  http://www.semanticweb.org/exam-example#isIssueOf
:isIssueOf rdf:type owl:ObjectProperty ,
                    owl:FunctionalProperty ;
           rdfs:domain :JournalVolume ;
           rdfs:range :Journal ;
           rdfs:comment "isIssueOf relates a journal volume to its journal." .


###  http://www.semanticweb.org/exam-example#isPartOf
:isPartOf rdf:type owl:ObjectProperty ,
                   owl:TransitiveProperty ,
                   owl:ReflexiveProperty ;
          rdfs:comment "hasPart is a superproperty of: isSectionOf, isArticleOf, isAbstractOf." .


###  http://www.semanticweb.org/exam-example#isPublishedBy
:isPublishedBy rdf:type owl:ObjectProperty ;
               owl:inverseOf :publishes ;
               rdf:type owl:FunctionalProperty ;
               rdfs:domain :ScientificPublication ;
               rdfs:range :Publisher ;
               rdfs:comment "isPublishedBy relates a journal to its publisher." .


###  http://www.semanticweb.org/exam-example#isSectionOf
:isSectionOf rdf:type owl:ObjectProperty ;
             rdfs:subPropertyOf :isPartOf ;
             rdfs:domain :Section ;
             rdfs:range :Article ;
             rdfs:comment "isSectionOf is a subproperty of isPartOf and relates a section to its article." .


###  http://www.semanticweb.org/exam-example#isUsedBy
:isUsedBy rdf:type owl:ObjectProperty ;
          owl:inverseOf :usesRepository ;
          rdf:type owl:InverseFunctionalProperty ;
          rdfs:domain :OpenAccessRepository ;
          rdfs:range :Publisher ;
          rdfs:comment "isUsedBy relates a repository to the publisher that uses it." .


###  http://www.semanticweb.org/exam-example#publishes
:publishes rdf:type owl:ObjectProperty ,
                    owl:InverseFunctionalProperty ;
           rdfs:domain :Publisher ;
           rdfs:range :Journal ;
           rdfs:comment "isPublishedBy relates a publisher to the journals published by it." .


###  http://www.semanticweb.org/exam-example#refersTo
:refersTo rdf:type owl:ObjectProperty ;
          rdfs:subPropertyOf owl:topObjectProperty ;
          rdfs:domain :References ;
          rdfs:range :Article .


###  http://www.semanticweb.org/exam-example#usesRepository
:usesRepository rdf:type owl:ObjectProperty ,
                         owl:FunctionalProperty ;
                rdfs:domain :Publisher ;
                rdfs:range :OpenAccessRepository ;
                rdfs:comment "usesRepository relates a publisher to an open access repository used by it." .


#################################################################
#    Data properties
#################################################################

###  http://www.semanticweb.org/exam-example#hasDate
:hasDate rdf:type owl:DatatypeProperty ;
         rdfs:subPropertyOf owl:topDataProperty ;
         rdf:type owl:FunctionalProperty ;
         rdfs:domain :JournalVolume ;
         rdfs:range xsd:dateTime ;
         rdfs:comment "hasDate relates a journal volume and the date of the publication." .


###  http://www.semanticweb.org/exam-example#hasNumber
:hasNumber rdf:type owl:DatatypeProperty ,
                    owl:FunctionalProperty ;
           rdfs:domain :JournalVolume ;
           rdfs:range xsd:nonNegativeInteger ;
           rdfs:comment "hasNumber relates a journal volume and its identified number." .


#################################################################
#    Classes
#################################################################

###  http://www.semanticweb.org/exam-example#Abstract
:Abstract rdf:type owl:Class ;
          rdfs:comment "An abstract is a brief summary of the content of an article. It is part of the article." .


###  http://www.semanticweb.org/exam-example#Article
:Article rdf:type owl:Class ;
         rdfs:subClassOf :ScientificPublication ,
                         [ rdf:type owl:Restriction ;
                           owl:onProperty :hasAbstract ;
                           owl:allValuesFrom :Abstract
                         ] ,
                         [ rdf:type owl:Restriction ;
                           owl:onProperty :hasSection ;
                           owl:allValuesFrom :Section
                         ] ,
                         [ rdf:type owl:Restriction ;
                           owl:onProperty :hasSection ;
                           owl:minQualifiedCardinality "4"^^xsd:nonNegativeInteger ;
                           owl:onClass :Section
                         ] ,
                         [ rdf:type owl:Restriction ;
                           owl:onProperty :hasAbstract ;
                           owl:qualifiedCardinality "1"^^xsd:nonNegativeInteger ;
                           owl:onClass :Abstract
                         ] ,
                         [ rdf:type owl:Restriction ;
                           owl:onProperty :hasSection ;
                           owl:qualifiedCardinality "1"^^xsd:nonNegativeInteger ;
                           owl:onClass :Conclusions
                         ] ,
                         [ rdf:type owl:Restriction ;
                           owl:onProperty :hasSection ;
                           owl:qualifiedCardinality "1"^^xsd:nonNegativeInteger ;
                           owl:onClass :Introduction
                         ] ,
                         [ rdf:type owl:Restriction ;
                           owl:onProperty :hasSection ;
                           owl:qualifiedCardinality "1"^^xsd:nonNegativeInteger ;
                           owl:onClass :References
                         ] ;
         rdfs:comment "An article can be a conference article or a journal article." .


###  http://www.semanticweb.org/exam-example#Conclusions
:Conclusions rdf:type owl:Class ;
             rdfs:subClassOf :Section ;
             rdfs:comment "The Conclusions are a section of an article." .


###  http://www.semanticweb.org/exam-example#ConferenceArticle
:ConferenceArticle rdf:type owl:Class ;
                   rdfs:subClassOf :Article ;
                   owl:disjointWith :JournalArticle ;
                   rdfs:comment "A conference article is an article published in the context of a conference. It has to have an abstract and at least the following sections: Introduction, Conclusions, References." .


###  http://www.semanticweb.org/exam-example#Introduction
:Introduction rdf:type owl:Class ;
              rdfs:subClassOf :Section ;
              rdfs:comment "The Introduction is a section of an article." .


###  http://www.semanticweb.org/exam-example#Journal
:Journal rdf:type owl:Class ;
         rdfs:subClassOf :ScientificPublication ,
                         [ rdf:type owl:Restriction ;
                           owl:onProperty :isPublishedBy ;
                           owl:qualifiedCardinality "1"^^xsd:nonNegativeInteger ;
                           owl:onClass :Publisher
                         ] ;
         rdfs:comment "A journal consists of one or more journal volumes." .


###  http://www.semanticweb.org/exam-example#JournalArticle
:JournalArticle rdf:type owl:Class ;
                owl:equivalentClass [ owl:intersectionOf ( :Article
                                                           [ rdf:type owl:Restriction ;
                                                             owl:onProperty :isArticleOf ;
                                                             owl:someValuesFrom :JournalVolume
                                                           ]
                                                         ) ;
                                      rdf:type owl:Class
                                    ] ;
                rdfs:subClassOf :Article ;
                rdfs:comment "A journal article is an article published in a journal volume. It has to have an abstract and at least the following sections: Introduction, Conclusions, References. A journal article can be the extended version of a conference article." .


###  http://www.semanticweb.org/exam-example#JournalVolume
:JournalVolume rdf:type owl:Class ;
               rdfs:subClassOf :ScientificPublication ,
                               [ rdf:type owl:Restriction ;
                                 owl:onProperty :hasArticle ;
                                 owl:allValuesFrom :JournalArticle
                               ] ,
                               [ rdf:type owl:Restriction ;
                                 owl:onProperty :hasArticle ;
                                 owl:minQualifiedCardinality "5"^^xsd:nonNegativeInteger ;
                                 owl:onClass :JournalArticle
                               ] ,
                               [ rdf:type owl:Restriction ;
                                 owl:onProperty :isIssueOf ;
                                 owl:qualifiedCardinality "1"^^xsd:nonNegativeInteger ;
                                 owl:onClass :Journal
                               ] ,
                               [ rdf:type owl:Restriction ;
                                 owl:onProperty :hasDate ;
                                 owl:qualifiedCardinality "1"^^xsd:nonNegativeInteger ;
                                 owl:onDataRange xsd:dateTime
                               ] ,
                               [ rdf:type owl:Restriction ;
                                 owl:onProperty :hasNumber ;
                                 owl:qualifiedCardinality "1"^^xsd:nonNegativeInteger ;
                                 owl:onDataRange xsd:nonNegativeInteger
                               ] ;
               rdfs:comment "A journal volume is an issue of a journal and consists of at least one journal article." ;
               rdfs:label "Journal Volume"@en .


###  http://www.semanticweb.org/exam-example#OpenAccessRepository
:OpenAccessRepository rdf:type owl:Class ;
                      rdfs:comment "An open access repository collects articles and provides free access to them." .


###  http://www.semanticweb.org/exam-example#Publisher
:Publisher rdf:type owl:Class ;
           rdfs:subClassOf [ rdf:type owl:Restriction ;
                             owl:onProperty :usesRepository ;
                             owl:qualifiedCardinality "1"^^xsd:nonNegativeInteger ;
                             owl:onClass :OpenAccessRepository
                           ] ;
           rdfs:comment "A publisher is an organization that publishes journals." .


###  http://www.semanticweb.org/exam-example#References
:References rdf:type owl:Class ;
            rdfs:subClassOf :Section ,
                            [ rdf:type owl:Restriction ;
                              owl:onProperty :refersTo ;
                              owl:someValuesFrom :Article
                            ] ;
            rdfs:comment "The References are a section of an article." .


###  http://www.semanticweb.org/exam-example#ScientificPublication
:ScientificPublication rdf:type owl:Class ;
                       rdfs:comment "A scientific publication can be a journal, a journal volume or an article." .


###  http://www.semanticweb.org/exam-example#Section
:Section rdf:type owl:Class ;
         rdfs:comment "A section is a part of an article. Example of sections can be Introduction, Conclusions and References." .


#################################################################
#    General axioms
#################################################################

[ rdf:type owl:AllDisjointClasses ;
  owl:members ( :Abstract
                :OpenAccessRepository
                :Publisher
                :ScientificPublication
                :Section
              )
] .


[ rdf:type owl:AllDisjointClasses ;
  owl:members ( :Article
                :Journal
                :JournalVolume
              )
] .


[ rdf:type owl:AllDisjointClasses ;
  owl:members ( :Conclusions
                :Introduction
                :References
              )
] .


###  Generated by the OWL API (version 4.5.9.2019-02-01T07:24:44Z) https://github.com/owlcs/owlapi